refine Solver.v.

FindVal.v
@@ -3,6 +3,7 @@ Require Import Lists.ListSet.
 Require Import Lists.List.
 Import Lists.List.ListNotations. 
 
+(** Collect different variables into a list set.*)
 Fixpoint collect_var (p : form) : (set id):=
   match p with
   | var i => (set_add  id_eq_dec i nil)
@@ -23,75 +24,18 @@ Compute (set_add id_eq_dec (Id "x") nil).
  
 Eval compute in (collect_var (land (lor x (not y)) (lor (not x) y))).
 
-
-
 End Test_collect_var.
 
 
-(*
-Can't defined in the following generator way
-
-Fixpoint next_valuation (V : valuation) (l : list id) : option valuation :=
-  match l with
-  | nil => None
-  | x::xs => if negb (V x)
-             then Some (override V x true)
-             else next_valuation (override V x false) xs
-  end.
-
-Module Test''.
-
- Definition x := (Id "x").
- Definition y := (Id "y").
- Definition z := (Id "z").
- 
- Definition apply_test (ov : option valuation) (i :id) :option Datatypes.bool :=
-   match ov with
-   |Some v => Some (v i)
-   |None => None
-   end.
-
- Fixpoint apply_list  (ov : option valuation) (l :list id) : list (option Datatypes.bool):=
-   match l with 
-   |nil => []
-   | x :: xs => (apply_test ov x) :: (apply_list ov xs)
-   end.
- 
-Eval compute in (apply_list (next_valuation (override (override (override empty_valuation x true) y false)z true ) [x;y;z]) [x;y;z]).
-
-Fixpoint all_valuation (V : option valuation) (l: list id) (n : nat) : list (list (option Datatypes.bool)):=
-  match n with
-  | 0 => []
-  | S n' =>
-    match V with
-    |Some v => (apply_list V l) :: (all_valuation (next_valuation v l) l n')
-    |None => []
-    end
-  end.
-
-
-
-Eval compute in (all_valuation (Some empty_valuation) [x;y;z] 10).
-
-End Test''.
-
-Fixpoint try_valuation (v: valuation) (p:form) (l :list id) : option valuation :=
-  if interp v p
-  then Some v
-  else match (next_valuation v l) with
-       | None => None
-       | Some v' => try_valuation v' p l
-       end.
-Error!
-*)
-
-
+(** Add a new id into the enum of valuation for k ids, ruturn enum of valuation for k+1 ids.*)
 Fixpoint add_id (lv: list valuation) (i:id) : list valuation :=
    match lv with
   | nil => []
   | v::vs => [(override v i true);(override v i false)] ++ (add_id vs i)
+   (*for each v, we add a true and a false, get two new v_s.*)
    end.
 
+(** Generate a enum of valuation from a list of ids.*)
 Fixpoint enum_valuation (l : list id) : list valuation :=
   match l with
   | nil => [empty_valuation]
@@ -104,14 +48,14 @@ Module Test_enum_valuation.
  Definition y := (Id "y").
  Definition z := (Id "z").
 
- 
-
- Fixpoint apply_list  (v : valuation) (l :list id) : list Datatypes.bool:=
+(** Get bool values of a list of variables from a valuation. *)
+ Fixpoint apply_list  (v : valuation) (l :list id) : list bool:=
    match l with 
    |nil => []
    | x :: xs => (v x) :: (apply_list v xs)
    end.
 
+(** Show values of a list of variables from a list of valuations.*) 
  Fixpoint all_valuations (lv : list valuation) (l: list id) : list (list Datatypes.bool):=
     match lv with
     |nil => []
@@ -124,6 +68,7 @@ Module Test_enum_valuation.
  Eval compute in (all_valuations (enum_valuation [x;y;z]) [x;y;z]).
 End Test_enum_valuation.
 
+(** Try to interpret a formula with a list of valuations, if one of them makes formula true, return it.*)
 Fixpoint try_valuation (lv: list valuation) (p : form) : option valuation :=
   match lv with
   | nil => None
@@ -132,6 +77,11 @@ Fixpoint try_valuation (lv: list valuation) (p : form) : option valuation :=
   end.
 
 
+(** Exercise 2.5*)
+(** 
+    Find a possible valuation that makes formual true.
+    Collect variables, generate all valuations and try them.
+**)
 Definition find_valuation (p : form) : option valuation :=
   let ids := collect_var p in
   let vals := (enum_valuation ids) in
@@ -147,16 +97,16 @@ Module Test_find_valuation.
    |None => None
    end.
 
-Fixpoint apply_list  (ov : option valuation) (l :list id) : list (option Datatypes.bool):=
+ Fixpoint apply_list  (ov : option valuation) (l :list id) : list (option Datatypes.bool):=
    match l with 
    |nil => []
    | x :: xs => (apply_test ov x) :: (apply_list ov xs)
    end.
-
-Definition find_valuation' (p : form) : list (option Datatypes.bool) :=
-  let ids := collect_var p in
-  let vals := (enum_valuation ids) in
-  apply_list (try_valuation vals p) ids.
+ (**A variant that can show values in the found valuation.*)
+ Definition find_valuation' (p : form) : list (option Datatypes.bool) :=
+   let ids := collect_var p in
+   let vals := (enum_valuation ids) in
+   apply_list (try_valuation vals p) ids.
  
  Eval compute in (find_valuation' (land (land x (not x)) (boolv true))). 
 
