Solver.v
@@ -1,18 +1,46 @@
-Require Import Formula Find.
-From Coq Require Import Lists.ListSet.
-From Coq Require Import Strings.String.
-Import ListNotations.
+Require Import Formula FindVal.
 Require Setoid. 
 
 
-Definition solver (p : form) :Datatypes.bool:=
+(** Pure SAT solver. *)
+Definition solver (p : form) :bool:=
   match find_valuation p with
   | Some _ => true
   | None => false
   end.
 
+(** Exercise 2.6*)
+(**
+   Difference between satisfiable and solver.
+   satisfiable is a property of a boolean formula, solver is a method to find out whether a formula is satisfiable. If solver returns true then we can conclude that the formula is satisfiable.
+ **)
 
+Module Test_solver.
+  Definition x := (var (Id "x")).
+  Definition y := (var (Id "y")).
 
+(** Exercise 2.7*)
+  Lemma test_pos_1: solver (land (lor x (not y)) (lor (not x) y) ) =true.
+  Proof.
+    reflexivity.
+  Qed.
+  
+  Lemma test_pos_2: solver (mapsto (not y) (lor x y) ) =true.  
+  Proof.
+    reflexivity.
+  Qed.
+  
+  Lemma test_neg_1: solver (land (land x (not x)) (boolv true)) = false.
+  Proof.
+    reflexivity.
+  Qed.
+  
+  Lemma test_neg_2: solver (land  (not x) (boolv false)) = false.
+  Proof.
+    reflexivity.
+  Qed.
+     
+End Test_solver.
 
 (*
 Lemma find_val_rec : forall p v v' l, interp v p = true \/ (interp v p = false /\ try_valuation l p= Some v' ) ->  (exists V, try_valuation (v::l) p=Some V).
@@ -51,84 +79,80 @@ Proof.
 Qed.*)
 
 
-Lemma land_find_interp: forall p1 p2 V, find_valuation (land p1 p2)=Some V -> interp V p1=true /\ interp V p2=true.
+Lemma find_interp_land: forall p1 p2 V, find_valuation (land p1 p2)=Some V -> interp V p1=true /\ interp V p2=true.
 Proof.
   intros.
-  split;unfold find_valuation in H;
-    unfold try_valuation in H;
-    induction (enum_valuation (collect_var (land p1 p2)));
-    try(discriminate H);
-    try(  destruct (interp a (land p1 p2)) eqn: E1);
-    
-       try(inversion H;
-         apply land_interp_interp in E1;
-         destruct E1;
-         rewrite <-H1;
-         assumption);
-       try(apply IHl; (*why it works?*)
-         apply H).
+  unfold find_valuation in H.
+  unfold try_valuation in H.
+  induction (enum_valuation (collect_var (land p1 p2))).
+  - discriminate H. (*valuation list is empty*)
+  - destruct (interp a (land p1 p2)) eqn: E1.
+    + inversion H. (* interp a (land p1 p2) = true => a = V*)
+      apply split_interp_land in E1.
+      (*split  (interp a (land p1 p2)) into  (interp a  p1) and (interp a  p2)*)
+      rewrite H1 in E1.
+      assumption.
+    + apply IHl. (* interp a (land p1 p2) = false*)
+      apply H. (* use hypothesis from induction*)
 Qed.
 
 
 
-Lemma lor_find_interp: forall p1 p2 V, find_valuation (lor p1 p2)=Some V -> interp V p1=true \/ interp V p2=true.
+Lemma find_interp_lor: forall p1 p2 V, find_valuation (lor p1 p2)=Some V -> interp V p1=true \/ interp V p2=true.
 Proof.
   intros.
-  unfold find_valuation in H;
-    unfold try_valuation in H;
-    induction (enum_valuation (collect_var (lor p1 p2))).
-    - discriminate H.
-    - destruct (interp a (lor p1 p2)) eqn: E1.
-    
-       + inversion H.
-         apply lor_interp_interp in E1.
-         rewrite <-H1;
-           assumption.
-         
-     +   try(apply IHl; (*why it works?*)
-         apply H).
+  unfold find_valuation in H.
+  unfold try_valuation in H.
+  induction (enum_valuation (collect_var (lor p1 p2))).
+  - discriminate H. (*valuation list is empty*)
+  - destruct (interp a (lor p1 p2)) eqn: E1.
+    + inversion H. (* interp a (lor p1 p2) = true => a = V*)
+      apply split_interp_lor in E1.
+      (*split  (interp a (lor p1 p2)) into  (interp a  p1) and (interp a  p2)*)
+      rewrite H1 in E1.
+      assumption.
+    + apply IHl. (* interp a (lor p1 p2) = false*)
+      apply H. (* use hypothesis from induction*)
 Qed.
 
 
 
-Lemma mapsto_find_interp: forall p1 p2 V, find_valuation (mapsto p1 p2)=Some V -> interp V p1=false \/ interp V p2=true.
+Lemma find_interp_mapsto: forall p1 p2 V, find_valuation (mapsto p1 p2)=Some V -> interp V p1=false \/ interp V p2=true.
 Proof.
   intros.
-  unfold find_valuation in H;
-    unfold try_valuation in H;
-    induction (enum_valuation (collect_var (mapsto p1 p2))).
-    - discriminate H.
-    - destruct (interp a (mapsto p1 p2)) eqn: E1.
-    
-       + inversion H.
-         apply mapsto_interp_interp in E1.
-         rewrite <-H1;
-           assumption.
-         
-     +   try(apply IHl; (*why it works?*)
-         apply H).
-Qed.
+  unfold find_valuation in H.
+  unfold try_valuation in H.
+  induction (enum_valuation (collect_var (mapsto p1 p2))).
+  - discriminate H. (*valuation list is empty*)
+  - destruct (interp a (mapsto p1 p2)) eqn: E1.
+    + inversion H. (* interp a (mapsto p1 p2) = true => a = V*)
+      apply split_interp_mapsto in E1.
+      (*split  (interp a (mapsto p1 p2)) into  (interp a  p1) and (interp a  p2)*)
+      rewrite H1 in E1.
+      assumption.
+    + apply IHl. (* interp a (lor p1 p2) = false*)
+      apply H. (* use hypothesis from induction*)
+Qed. 
 
 
 
-
-Lemma not_find_interp: forall p V, find_valuation (not p)=Some V -> interp V p=false.
+Lemma find_interp_not: forall p V, find_valuation (not p)=Some V -> interp V p=false.
 Proof.
   intros.
-  unfold find_valuation in H;
-    unfold try_valuation in H;
-    induction (enum_valuation (collect_var (not p))).
-    - discriminate H.
-    - destruct (interp a (not p)) eqn: E1.
-    
-       + inversion H.
-         apply not_interp_interp in E1.
-         rewrite <-H1;
-           assumption.
-         
-     +   try(apply IHl; (*why it works?*)
-         apply H).
+  unfold find_valuation in H.
+  unfold try_valuation in H.
+  induction (enum_valuation (collect_var (not p))).
+  - discriminate H. (*valuation list is empty*)
+  - destruct (interp a (not p)) eqn: E1.
+    + inversion H. (* interp a (land p1 p2) = true => a = V*)
+      apply split_interp_not in E1.
+      (*split  (interp a (not p)) into  (interp a  p) *)
+      rewrite H1 in E1.
+      assumption.
+    + apply IHl. (* interp a (mapsto p1 p2) = false*)
+      apply H. (* use hypothesis from induction*)
 Qed.
+  
 
 (*
 Lemma and_satisfiable : forall p1 p2, satisfiable p1 -> satisfiable p2 -> satisfiable (land p1 p2).
@@ -144,46 +168,52 @@ didn't work because the lemma is false!
   
   
   
-  
 Lemma solver_sound : forall p, solver p = true -> satisfiable p.
 Proof.
   intros.
-  destruct p;unfold satisfiable;unfold solver in H.
+  destruct p; (* not induction*)
+    unfold satisfiable;
+    unfold solver in H.
   - (*var*)
-    exists (override empty_valuation i true).
+    exists (override empty_valuation i true). (* find a witness*)
     simpl.
     unfold override.
-    now rewrite  <- beq_id_refl.
+    now rewrite  <-  eqb_id_refl.
   - (*bool*)
-    destruct (find_valuation (bool b)) eqn:E in H;(try discriminate H).
+    destruct (find_valuation (boolv b)) eqn:E in H;
+      (try discriminate H).
     unfold find_valuation in E.  
     simpl in E.
     destruct b.    
     now exists v.
     discriminate E.
   -  (*land*)
-    destruct (find_valuation (land p1 p2)) eqn:E in H;(try discriminate H).
+    destruct (find_valuation (land p1 p2)) eqn:E in H;
+      (try discriminate H).
     exists v.
-    apply land_interp_interp.
-    apply land_find_interp in E.
+    apply split_interp_land.
+    apply find_interp_land in E.
     assumption.
   - (*lor*)
-    destruct (find_valuation (lor p1 p2)) eqn:E in H;try(discriminate H).
+    destruct (find_valuation (lor p1 p2)) eqn:E in H;
+      try(discriminate H).
     exists v.
-    apply lor_interp_interp.
-    apply lor_find_interp in E.
+    apply split_interp_lor.
+    apply find_interp_lor in E.
     assumption.
   - (* mapsto*)   
-    destruct (find_valuation (mapsto p1 p2)) eqn:E in H;try(discriminate H).
+    destruct (find_valuation (mapsto p1 p2)) eqn:E in H;
+      try(discriminate H).
     exists v.
-    apply mapsto_interp_interp.
-    apply mapsto_find_interp in E.
+    apply split_interp_mapsto.
+    apply find_interp_mapsto in E.
     assumption.
   - (* not*)   
-    destruct (find_valuation (not p)) eqn:E in H;try(discriminate H).
+    destruct (find_valuation (not p)) eqn:E in H;
+      try(discriminate H).
     exists v.
-    apply not_interp_interp.
-    apply not_find_interp in E.
+    apply split_interp_not.
+    apply find_interp_not in E.
     assumption.
 Qed.
 
